feat: Std.Data.HashMap: part 6 (proof of filterMap)

Std/Data/HashMap/Basic.lean
@@ -187,20 +187,20 @@ Applies `f` to each key-value pair `a, b` in the map. If it returns `some c` the
 -/
 @[specialize] def filterMap {α : Type u} {β : Type v} {γ : Type w}
     (f : α → β → Option γ) (m : Imp α β) : Imp α γ :=
-  let m' := m.buckets.1.mapM (m := StateT (ULift Nat) Id) (go · · .nil) |>.run ⟨0⟩ |>.run
+  let m' := m.buckets.1.mapM (m := StateT (ULift Nat) Id) (go .nil) |>.run ⟨0⟩ |>.run
   have : m'.1.size > 0 := by
-    have := Array.size_mapM (m := StateT (ULift Nat) Id) (go · · .nil) m.buckets.1
+    have := Array.size_mapM (m := StateT (ULift Nat) Id) (go .nil) m.buckets.1
     simp [SatisfiesM_StateT_eq, SatisfiesM_Id_eq] at this
     simp [this, Id.run, StateT.run, m.2.2]
   ⟨m'.2.1, m'.1, this⟩
 where
   /-- Inner loop of `filterMap`. Note that this reverses the bucket lists,
   but this is fine since bucket lists are unordered. -/
-  @[specialize] go : AssocList α β → ULift Nat → AssocList α γ → AssocList α γ × ULift Nat
-  | .nil, n, acc => (acc, n)
-  | .cons a b l, n, acc => match f a b with
-    | none => go l n acc
-    | some c => go l ⟨n.1 + 1⟩ (.cons a c acc)
+  @[specialize] go (acc : AssocList α γ) : AssocList α β → ULift Nat → AssocList α γ × ULift Nat
+  | .nil, n => (acc, n)
+  | .cons a b l, n => match f a b with
+    | none => go acc l n
+    | some c => go (.cons a c acc) l ⟨n.1 + 1⟩
 
 /-- Constructs a map with the set of all pairs `a, b` such that `f` returns true. -/
 @[inline] def filter (f : α → β → Bool) (m : Imp α β) : Imp α β :=
@@ -298,20 +298,6 @@ instance : GetElem (HashMap α β) α (Option β) fun _ _ => True where
 
 /-- Returns true if the element `a` is in the map. -/
 @[inline] def contains (self : HashMap α β) (a : α) : Bool := self.1.contains a
-
-private unsafe def filterMapImpl (f : α → β → Option γ) (self : HashMap α β) : HashMap α γ :=
-  ⟨self.1.filterMap f, lcProof⟩ -- FIXME: add proof
-
-/--
-Applies `f` to each key-value pair `a, b` in the map. If it returns `some c` then
-`a, c` is pushed into the new map; else the key is removed from the map.
--/
-@[implementedBy filterMapImpl]
-opaque filterMap (f : α → β → Option γ) (self : HashMap α β) : HashMap α γ
-
-/-- Constructs a map with the set of all pairs `a, b` such that `f` returns true. -/
-@[inline] def filter (f : α → β → Bool) (self : HashMap α β) : HashMap α β :=
-  self.filterMap fun a b => bif f a b then some b else none
 
 /-- Folds a monadic function over the elements in the map (in arbitrary order). -/
 @[inline] def foldM [Monad m] (f : δ → α → β → m δ) (init : δ) (self : HashMap α β) : m δ :=
